Simple_Networks/Simple_Network_Language_Certificate_Checking.thy
@@ -1,7 +1,7 @@
 theory Simple_Network_Language_Certificate_Checking
   imports
     "../Normalized_Zone_Semantics_Certification_Impl"
-    Simple_Network_Language_Model_Checking
+    Simple_Network_Language_Export_Code
 begin
 
 (* XXX Merge proof with Ex_ev *)
@@ -49,20 +49,6 @@ sublocale impl: Reachability_Problem_Impl_Precise
   and states_mem_impl = states'_memi
   by standard (unfold PR_CONST_def, rule impl.E_precise_op'_impl.refine, rule states'_memi_correct)
 
-definition
-  "unreachability_checker L_list M_list \<equiv>
-  let
-    Fi = impl.F_impl';
-    Pi = impl.P_impl;
-    copyi = amtx_copy;
-    Lei = dbm_subset_impl m;
-    l\<^sub>0i = return l\<^sub>0i;
-    s\<^sub>0i = impl.init_dbm_impl;
-    succsi = impl.succs_precise'_impl;
-    M_table = impl.M_table M_list
-  in
-  certify_unreachable_impl Fi Pi copyi Lei l\<^sub>0i s\<^sub>0i succsi L_list M_table"
-
 lemma state_impl_abstract':
   assumes "states'_memi li"
   shows "\<exists>l. (li, l) \<in> loc_rel"
@@ -72,10 +58,6 @@ proof -
   with state_impl_abstract[of Li si] show ?thesis
     using assms unfolding states'_memi_def states_def by auto
 qed
-
-lemmas unreachability_checker_hnr' =
-  impl.certify_unreachable_impl_hnr[folded unreachability_checker_def[unfolded Let_def],
-    OF state_impl_abstract']
 
 interpretation Bisimulation_Invariant
   "(\<lambda>(l, u) (l', u'). conv_A prod_ta \<turnstile>' \<langle>l, u\<rangle> \<rightarrow> \<langle>l', u'\<rangle>)"
@@ -118,38 +100,141 @@ theorem unreachability_checker_hnr:
     and "fst ` set M_list \<subseteq> set L_list"
     and "formula = formula.EX \<phi>"
   shows "(
-  uncurry0 (unreachability_checker L_list M_list),
+  uncurry0 (impl.unreachability_checker L_list M_list),
   uncurry0 (SPEC (\<lambda>r. r \<longrightarrow>
     \<not> Simple_Network_Language.conv A,(L\<^sub>0, map_of s\<^sub>0, \<lambda>_. 0) \<Turnstile> formula)))
   \<in> unit_assn\<^sup>k \<rightarrow>\<^sub>a bool_assn"
-  supply [sep_heap_rules] =
-    unreachability_checker_hnr'[OF assms(1-3), to_hnr, unfolded hn_refine_def, rule_format]
-  using unreachability_prod[OF assms(4)] by sepref_to_hoare (sep_auto simp: pure_def)
+proof -
+  define checker where "checker \<equiv> impl.unreachability_checker L_list M_list"
+  note [sep_heap_rules] =
+    impl.unreachability_checker_hnr[
+      OF state_impl_abstract', OF assms(1-3),
+      to_hnr, unfolded hn_refine_def, rule_format, folded checker_def
+    ]
+  show ?thesis
+    unfolding checker_def[symmetric] using unreachability_prod[OF assms(4)]
+    by sepref_to_hoare (sep_auto simp: pure_def)
+qed
+
+schematic_goal succs_impl_alt_def:
+  "impl.succs_precise'_impl \<equiv> ?impl"
+  unfolding impl.succs_precise'_impl_def impl.succs_precise_inner_impl_def
+  apply (abstract_let impl.E_precise_op'_impl E_op_impl)
+  unfolding impl.E_precise_op'_impl_def fw_impl'_int
+  apply (abstract_let trans_impl trans_impl)
+  unfolding trans_impl_def
+  apply (abstract_let int_trans_impl int_trans_impl)
+  apply (abstract_let bin_trans_from_impl bin_trans_impl)
+  apply (abstract_let broad_trans_from_impl broad_trans_impl)
+  unfolding int_trans_impl_def bin_trans_from_impl_def broad_trans_from_impl_def
+  apply (abstract_let trans_in_broad_grouped trans_in_broad_grouped)
+  apply (abstract_let trans_out_broad_grouped trans_out_broad_grouped)
+  apply (abstract_let trans_in_map trans_in_map)
+  apply (abstract_let trans_out_map trans_out_map)
+  apply (abstract_let int_trans_from_all_impl int_trans_from_all_impl)
+  unfolding int_trans_from_all_impl_def
+  apply (abstract_let int_trans_from_vec_impl int_trans_from_vec_impl)
+  unfolding int_trans_from_vec_impl_def
+  apply (abstract_let int_trans_from_loc_impl int_trans_from_loc_impl)
+  unfolding int_trans_from_loc_impl_def
+  apply (abstract_let trans_i_map trans_i_map)
+  unfolding trans_out_broad_grouped_def trans_out_broad_map_def
+  unfolding trans_in_broad_grouped_def trans_in_broad_map_def
+  unfolding trans_in_map_def trans_out_map_def
+  unfolding trans_i_map_def
+  apply (abstract_let trans_map trans_map)
+  apply (abstract_let "inv_fun :: nat list \<times> int list \<Rightarrow> _" inv_fun)
+  unfolding inv_fun_alt_def
+  apply (abstract_let invs2 invs)
+  unfolding invs2_def
+  apply (abstract_let n_ps n_ps)
+  by (rule Pure.reflexive)
+
+context
+  fixes L_list and M_list :: "((nat list \<times> int list) \<times> int DBMEntry list list) list"
+  assumes assms:
+    "list_all states'_memi L_list"
+    "fst ` set M_list \<subseteq> set L_list"
+begin
+
+private lemma A:
+  "list_all (\<lambda>x. states'_memi x \<and> states'_memi x) L_list"
+  using assms by simp
+
+schematic_goal unreachability_checker_alt_def:
+  "impl.unreachability_checker L_list M_list \<equiv> ?x"
+  apply (subst
+      impl.unreachability_checker_def[OF state_impl_abstract', of states'_memi, OF _ A assms(2)])
+     apply assumption
+  apply (subst impl.M_table_def[OF state_impl_abstract', of states'_memi, OF _ A assms(2)])
+   apply assumption
+  unfolding impl.F_impl'_def impl.P_impl_def
+  apply (abstract_let states'_memi check_states)
+  unfolding states'_memi_def states_mem_compute'
+  apply (abstract_let "map states_i [0..<n_ps]" states_i)
+  unfolding succs_impl_alt_def
+  unfolding k_impl_alt_def k_i_def
+  (* The following are just to unfold things that should have been defined in a defs locale *)
+  unfolding impl.E_op''_impl_def impl.abstr_repair_impl_def impl.abstra_repair_impl_def
+  unfolding
+    impl.start_inv_check_impl_def impl.unbounded_dbm_impl_def
+    impl.unbounded_dbm'_def
+  unfolding impl.init_dbm_impl_def impl.a\<^sub>0_impl_def
+  unfolding impl.subsumes_impl_def
+  unfolding impl.emptiness_check_impl_def
+  unfolding impl.state_copy_impl_def
+  by (rule Pure.reflexive)
+
+end (* Anonymous context *)
+
+thm states'_memi_def
 
 end (* Simple_Network_Impl_nat_ceiling_start_state *)
 
 concrete_definition unreachability_checker uses
-  Simple_Network_Impl_nat_ceiling_start_state.unreachability_checker_def
+  Simple_Network_Impl_nat_ceiling_start_state.unreachability_checker_alt_def
+
+lemma states'_memi_alt_def:
+  "Simple_Network_Impl_nat_defs.states'_memi broadcast bounds' automata = (
+     \<lambda>(L, s).
+    let
+      n_ps = length automata;
+      n_vs = Simple_Network_Impl.n_vs bounds';
+      states_i = map (Simple_Network_Impl_nat_defs.states_i automata) [0..<n_ps]
+    in
+      length L = n_ps \<and> (\<forall>i<n_ps. L ! i \<in> states_i ! i) \<and>
+      length s = n_vs \<and> Simple_Network_Impl_nat_defs.check_boundedi bounds' s
+    )
+    "
+  unfolding Simple_Network_Impl_nat_defs.states'_memi_def
+  unfolding Simple_Network_Impl_nat_defs.states_mem_compute'
+  unfolding Prod_TA_Defs.n_ps_def list_all_iff
+  by (intro ext) simp
 
 definition
   "certificate_checker
-    broadcast bounds' automata m num_states num_actions k L\<^sub>0 s\<^sub>0 formula M_list \<equiv>
+    M_list broadcast bounds' automata m num_states num_actions k L\<^sub>0 s\<^sub>0 formula \<equiv>
   let
     check1 = Simple_Network_Impl_nat_ceiling_start_state
       broadcast bounds' automata m num_states num_actions k L\<^sub>0 s\<^sub>0 formula;
     L_list = map fst M_list;
-    check2 = list_all (Simple_Network_Impl_nat_defs.states'_memi broadcast bounds' automata) L_list;
+    n_ps = length automata;
+    n_vs = Simple_Network_Impl.n_vs bounds';
+    states_i = map (Simple_Network_Impl_nat_defs.states_i automata) [0..<n_ps];
+    check2 = list_all (\<lambda>(L, s). length L = n_ps \<and> (\<forall>i<n_ps. L ! i \<in> states_i ! i) \<and>
+      length s = n_vs \<and> Simple_Network_Impl_nat_defs.check_boundedi bounds' s
+    ) L_list;
     check3 = (case formula of formula.EX _ \<Rightarrow> True | _ \<Rightarrow> False)
   in if check1 \<and> check2 \<and> check3 then
   do {
     r \<leftarrow> unreachability_checker
       broadcast bounds' automata m num_states num_actions L\<^sub>0 s\<^sub>0 formula L_list M_list;
-    return (Some r)
-  } else return None"
+    Heap_Monad.return (Some r)
+  } else Heap_Monad.return None"
 
 theorem certificate_check:
   "<emp> certificate_checker
-    broadcast bounds automata m num_states num_actions k L\<^sub>0 s\<^sub>0 formula M_list
+    M_list broadcast bounds automata m num_states num_actions k L\<^sub>0 s\<^sub>0 formula
    <\<lambda> Some r \<Rightarrow> \<up>(r \<longrightarrow> \<not> N broadcast automata bounds,(L\<^sub>0, map_of s\<^sub>0, \<lambda>_ . 0) \<Turnstile> formula)
     | None \<Rightarrow> true>\<^sub>t"
 proof -
@@ -164,11 +249,98 @@ proof -
         folded A_def check_def has_deadlock_def,
         to_hnr, unfolded hn_refine_def, rule_format,
         OF _ _ _ _ A, unfolded A]
-  } note *[sep_heap_rules] = this
+  } note *[sep_heap_rules] = this[simplified, unfolded hd_of_formulai.simps[abs_def]]
   show ?thesis
     unfolding A_def[symmetric] check_def[symmetric]
     unfolding certificate_checker_def
+    unfolding Let_def
+    unfolding states'_memi_alt_def[unfolded Let_def, symmetric, of automata bounds broadcast]
     by (sep_auto simp: unreachability_checker.refine[symmetric] pure_def split: formula.split_asm)
 qed
+
+definition rename_check where
+  "rename_check dc broadcast bounds' automata k L\<^sub>0 s\<^sub>0 formula
+    m num_states num_actions renum_acts renum_vars renum_clocks renum_states
+    (* inv_renum_states inv_renum_vars inv_renum_clocks *)
+    state_space
+\<equiv>
+do {
+  r \<leftarrow> do_rename_mc (
+      \<lambda>(show_clock :: (nat \<Rightarrow> string)) (show_state :: (nat list \<times> int list \<Rightarrow> char list)).
+      certificate_checker state_space)
+    dc broadcast bounds' automata k L\<^sub>0 s\<^sub>0 formula
+    m num_states num_actions renum_acts renum_vars renum_clocks renum_states
+    (* inv_renum_states inv_renum_vars inv_renum_clocks; *)
+    (\<lambda>_ _. '' '') (\<lambda>_. '' '') (\<lambda>_. '' '');
+  case r of Some r \<Rightarrow>
+    case r of
+      None \<Rightarrow> Heap_Monad.return Preconds_Unsat
+    | Some False \<Rightarrow> Heap_Monad.return Unsat
+    | Some True \<Rightarrow> Heap_Monad.return Sat
+  | None \<Rightarrow> Heap_Monad.return Renaming_Failed}
+"
+
+theorem certificate_check_rename:
+  "<emp> rename_check False broadcast bounds automata k L\<^sub>0 s\<^sub>0 formula
+    m num_states num_actions renum_acts renum_vars renum_clocks renum_states
+    (* inv_renum_states inv_renum_vars inv_renum_clocks *)
+    state_space
+    <\<lambda> Sat \<Rightarrow> \<up>(
+        (\<not> N broadcast automata bounds,(L\<^sub>0, map_of s\<^sub>0, \<lambda>_ . 0) \<Turnstile> formula))
+     | Renaming_Failed \<Rightarrow> \<up>(\<not> Simple_Network_Rename_Formula
+        broadcast bounds renum_vars renum_clocks renum_states automata formula s\<^sub>0 L\<^sub>0)
+     | Unsat \<Rightarrow> true
+     | Preconds_Unsat \<Rightarrow> true
+    >\<^sub>t"
+proof -
+  have *: "
+    Simple_Network_Rename_Formula_String
+        broadcast bounds renum_vars renum_clocks renum_states automata formula s\<^sub>0 L\<^sub>0
+  = Simple_Network_Rename_Formula
+        broadcast bounds renum_vars renum_clocks renum_states automata formula s\<^sub>0 L\<^sub>0
+  "
+    unfolding
+      Simple_Network_Rename_Formula_String_def Simple_Network_Rename_Formula_def
+      Simple_Network_Rename_def Simple_Network_Rename_Formula_axioms_def
+    using infinite_literal by auto
+  define A where "A \<equiv> N broadcast automata bounds"
+  define check where "check \<equiv> A,(L\<^sub>0, map_of s\<^sub>0, \<lambda>_ . 0) \<Turnstile> formula"
+  define A' where "A' \<equiv> N
+    (map renum_acts broadcast)
+    (map_index (renum_automaton renum_acts renum_vars renum_clocks renum_states) automata)
+    (map (\<lambda>(a,b,c). (renum_vars a, b, c)) bounds)"
+  define check' where "check' \<equiv>
+    A',(map_index renum_states L\<^sub>0, map_of (map (\<lambda>(x, v). (renum_vars x, v)) s\<^sub>0), \<lambda>_ . 0) \<Turnstile>
+    map_formula renum_states renum_vars id formula"
+  define renaming_valid where "renaming_valid \<equiv>
+    Simple_Network_Rename_Formula
+      broadcast bounds renum_vars renum_clocks renum_states automata formula s\<^sub>0 L\<^sub>0
+  "
+  have [simp]: "check \<longleftrightarrow> check'" 
+    if renaming_valid
+    using that unfolding check_def check'_def A_def A'_def renaming_valid_def
+    by (rule Simple_Network_Rename_Formula.models_iff'[symmetric])
+  note [sep_heap_rules] =
+    certificate_check[
+    of state_space
+    "map renum_acts broadcast" "map (\<lambda>(a,b,c). (renum_vars a, b, c)) bounds"
+    "map_index (renum_automaton renum_acts renum_vars renum_clocks renum_states) automata"
+    m num_states num_actions k "map_index renum_states L\<^sub>0" "map (\<lambda>(x, v). (renum_vars x, v)) s\<^sub>0"
+    "map_formula renum_states renum_vars id formula",
+    folded A'_def check'_def renaming_valid_def,
+    simplified
+    ]
+  show ?thesis
+    unfolding rename_check_def do_rename_mc_def rename_network_def
+    unfolding if_False
+    unfolding Simple_Network_Rename_Formula_String_Defs.check_renaming[symmetric] * Let_def
+    unfolding
+      A_def[symmetric] check_def[symmetric] renaming_valid_def[symmetric]
+    by (sep_auto simp: split: bool.splits)
+qed
+
+lemmas [code] = Simple_Network_Impl_nat_defs.states_i_def
+
+export_code rename_check in SML module_name Test
 
 end
